examples/iso_dh/proofs/responder.v
@@ -85,7 +85,8 @@ wp_apply (wp_mk_nonce_freshN {[ga]}
   rewrite minted_TInt /= bi.True_and.
   iModIntro. by iApply bi.equiv_iff.
   intro contra. destruct contra.
-iIntros "%b %fresh_b %nonce_b #m_b #s_b #dh_gb _ _ token".
+iIntros "%b %fresh_b #m_b #s_b #dh_gb _ _ token".
+have Nm_b : is_true (negb (is_mul (TNonce b))) by [].
 have {}fresh_b: ¬ subterm b ga by apply: fresh_b; exact/elem_of_singleton.
 rewrite bi.intuitionistic_intuitionistically.
 set gb := TExp (TInt 0) b.
@@ -97,9 +98,9 @@ rewrite (term_token_difference gb (↑iso_dhN.@"failed")); last by solve_ndisj.
 iDestruct "token" as "[token_failed token]".
 iPoseProof (term_token_difference gb (↑iso_dhN.@"res") with "token")
   as "[res_token token]"; first by solve_ndisj.
-iMod ("res" $! b with "res_token") as "[resI resR]".
+iMod ("res" $! (TNonce b) with "res_token") as "[resI resR]".
 iMod (iso_dh_ready_alloc N skI skR si with "[//] resI") as "#ready".
-iAssert (public gb) as "#p_gb"; first by iApply (public_dh_share (nonce_Nmul nonce_b)).
+iAssert (public gb) as "#p_gb"; first by iApply (public_dh_share Nm_b).
 wp_pure _ credit:"H1".
 wp_pure _ credit:"H2".
 wp_apply wp_mk_keyshare => //.
