examples/nsl_dh/proofs/responder.v
@@ -86,7 +86,7 @@ Lemma wp_responder_send_msg2 c skI skR ga N φ failed :
     failed_early skI skR failed
   }}}
     responder_send_msg2 c skR (Spec.pkey skI) (Tag N) ga
-  {{{ (b : term), RET (b, TExp (TInt 0) b);
+  {{{ (b : nonce), RET (TNonce b, TExp (TInt 0) b);
       let gb := TExp (TInt 0) b in
       let gab := TExp ga b in
       let si := SessInfo skI skR ga gb gab in
@@ -102,7 +102,7 @@ rewrite /responder_send_msg2.
 wp_pures. wp_apply wp_pkey. wp_pures.
 wp_apply (wp_mk_dh_keys {[ga]} skI skR); first by iFrame "#".
 { iIntros "%t %t_in". rewrite elem_of_singleton in t_in. by subst t. }
-iIntros "%b %fresh_b %nonce_b #dh_b rel ptok rtok res tok".
+iIntros "%b %fresh_b #dh_b rel ptok rtok res tok".
 have b_ga : ¬ subterm b ga.
 { apply: fresh_b. by rewrite elem_of_singleton. }
 set gb := TExp (TInt 0) b.
@@ -112,12 +112,12 @@ iMod (set_peer_share gb (Some ga) with "ptok") as "#ps_gb".
 (* Get φ from callback *)
 set gab := TExp ga b.
 set si := SessInfo skI skR ga gb gab.
-iMod ("φ_cb" $! b with "res") as "[φ_init φ_resp]".
+iMod ("φ_cb" $! (TNonce b) with "res") as "[φ_init φ_resp]".
 (* Allocate nsl_dh_ready *)
 iMod (nsl_dh_ready_alloc N skI skR si with "N_φ φ_init") as "#ready".
 (* Build and encrypt msg2 *)
 wp_list. wp_term_of_list. wp_pures.
-iDestruct "dh_b" as "(_ & #m_b & #s_b & #pred_b)".
+iDestruct "dh_b" as "(#m_b & #s_b & #pred_b)".
 wp_apply wp_aenc => //.
 { (* minted plaintext *)
   rewrite minted_of_list /= minted_pkey.
@@ -144,7 +144,7 @@ wp_apply wp_send => //. wp_pures.
 iApply ("Hpost" $! b). by iFrame "∗ #".
 Qed.
 
-Lemma wp_responder_recv_msg3 c skI skR ga b :
+Lemma wp_responder_recv_msg3 c skI skR ga (b : nonce) :
   let gb := TExp (TInt 0) b in
   let gab := TExp ga b in
   let si := SessInfo skI skR ga gb gab in
@@ -170,8 +170,8 @@ Proof.
 move=> gb gab si.
 iIntros "%Ψ (#chan & #ctx & #(m1_pred & m2_pred & m3_pred) &
          #m_skI & #m_skR & #m_ga & #s_ga & #dh_b & #ps_gb & rel) Hpost".
-iDestruct "dh_b" as "(%nonce_b & #m_b & #s_b & #pred_b)".
-have Nm_b : is_true (negb (is_mul b)) := nonce_Nmul nonce_b.
+iDestruct "dh_b" as "(#m_b & #s_b & #pred_b)".
+have Nm_b : is_true (negb (is_mul b)) by [].
 have Nm_b' : Is_true (negb (is_mul b)) := proj1 (is_trueP _) Nm_b.
 rewrite /responder_recv_msg3. wp_pures.
 wp_apply wp_pkey. wp_pures.
@@ -228,8 +228,7 @@ iDestruct "inv_m3" as "[#p_gb|(#inv_m3 & _)]".
       iApply public_TExp => //.
     * by iLeft.
 - (* msg3_pred — honest case *)
-  iPoseProof ("inv_m3" $! ga b with "[%] [%] ps_gb") as "[#rel_ga_gb #gab_iff]".
-  { done. }
+  iPoseProof ("inv_m3" $! ga b with "[%] ps_gb") as "[#rel_ga_gb #gab_iff]".
   { done. }
   wp_bind (derive_senc_key _). iApply wp_derive_senc_key. iNext. wp_pures.
   iApply ("Hpost" $! (Some (si_key si))). iRight. iModIntro. iSplit => //.
