examples/opaque/client_proofs.v
@@ -39,10 +39,10 @@ iIntros "%ϕ (#Cryptis & #Hpredrw & #HpredA_u & #HpredA_s & #HpredSK & #HpredK
   #Hfresh) Hhl".
 wp_lam; wp_pures.
 wp_apply (wp_mk_nonce_fresh fresh (fun _ => False)%I (fun t => opaque_secret t)%I) => //.
-iIntros "%x_u %Hfreshx_u %Hnoncex_u #Hmintedx_u #Hprivatex_u #Hexpx_u #? #Hexpx_uV Htokenx_u".
+iIntros "%x_u %Hfreshx_u #Hmintedx_u #Hprivatex_u #Hexpx_u #? #Hexpx_uV Htokenx_u".
 wp_pures.
 wp_apply (wp_mk_nonce_fresh fresh (fun _ => False)%I (fun _ => True)%I) => //.
-iIntros "%r %Hfreshr %Hnoncer #Hmintedr #Hprivater #Hexpr #HsrV #HexprV Htokenr".
+iIntros "%r %Hfreshr #Hmintedr #Hprivater #Hexpr #HsrV #HexprV Htokenr".
 wp_pures.
 wp_apply wp_H'; wp_apply wp_texp; wp_pures.
 wp_apply wp_texp; wp_list; wp_term_of_list; wp_pures.
@@ -52,7 +52,7 @@ wp_apply wp_send => //.
   do !iSplit => //.
   - iApply public_TExp_iff.
       by case.
-      by exact: (proj1 (is_trueP _) (nonce_Nmul Hnoncer)).
+      by exact: (proj1 (is_trueP _) (negb_is_mul_nonce r)).
     do !iSplit => //.
     + by rewrite minted_THash minted_tag.
     + iApply exp_pred_intro1.
@@ -61,14 +61,14 @@ wp_apply wp_send => //.
       by iApply (public_THashIS with "Hpredα") => //.
   - iApply public_TExp_iff.
       by case.
-      by exact: (proj1 (is_trueP _) (nonce_Nmul Hnoncex_u)).
+      by exact: (proj1 (is_trueP _) (negb_is_mul_nonce x_u)).
     do !iSplit => //.
     + by iApply minted_TInt.
     + iApply exp_pred_intro1.
       iApply "Hexpx_u"; iPureIntro.
-      have Nm : is_true (negb (is_mul x_u)) := nonce_Nmul Hnoncex_u.
-      rewrite (_ : TExp g x_u = TExpN g [x_u]); last by rewrite /TExpN TMulN1.
-      by rewrite exps_TExpN' //; [by case | by rewrite /atomic /= Nm | exact: (invs_canceled1 Nm)].
+      have Nm : is_true (negb (is_mul x_u)) := negb_is_mul_nonce x_u.
+      rewrite (_ : TExp g x_u = TExpN g [TNonce x_u]); last by rewrite /TExpN TMulN1.
+      by rewrite exps_TExpN'; [by [] | by case | by [] | exact: (invs_canceled1 Nm)].
     + by rewrite public_TInt; auto.
 wp_pures.
 wp_apply wp_recv => //.
@@ -78,7 +78,7 @@ wp_list_of_term m2; wp_pures => //.
   1: wp_list_match => [β X_s envelope A_s -> | _].
   1, 2: wp_pures.
   2, 3: by iApply ("Hhl" $! None); iModIntro; iSplit.
-wp_apply wp_hl_inv_term; first by exact: (nonce_Nmul Hnoncer).
+wp_apply wp_hl_inv_term; first by exact: (negb_is_mul_nonce r).
 wp_apply wp_texp; wp_list; wp_apply wp_H.
 wp_apply wp_derive_senc_key; set k := SEncKey _.
 wp_pures; wp_lam; wp_pures.
@@ -150,21 +150,21 @@ iModIntro; iSplit.
     rewrite public_of_list.
     iDestruct "contra" as "(contra & _ & _)".
     iDestruct "Hopaquepair" as
-        "(%p_s & -> & %Hfreshp_u & %Hnoncep_u & %Hnoncep_s & ? & ? & ? & ? & ? & ? & ?)".
+        "(%p_s & -> & %Hfreshp_u & ? & ? & ? & ? & ? & ? & ?)".
     rewrite TExp2_TExpN.
-    have p_u_s: p_u ≠ p_s.
+    have p_u_s: TNonce p_u ≠ TNonce p_s.
       move=> p_u_s; apply: Hfreshp_u; rewrite -p_u_s.
       apply/subtermsP.
-      rewrite (_ : TExp g p_u = TExpN g [p_u]); last by rewrite /TExpN TMulN1.
-      have Nm : is_true (negb (is_mul p_u)) := nonce_Nmul Hnoncep_u.
-      rewrite subtermsE //; last by rewrite /atomic /= Nm.
+      rewrite (_ : TExp g p_u = TExpN g [TNonce p_u]); last by rewrite /TExpN TMulN1.
+      have Nm : is_true (negb (is_mul p_u)) := negb_is_mul_nonce p_u.
+      rewrite subtermsE //.
       rewrite cancel_invs1 /=.
       by rewrite [subterms p_u]subterms_nonce //; set_solver.
-    have p_u_sV : p_u ≠ TInv p_s.
+    have p_u_sV : TNonce p_u ≠ TInv p_s.
       move=> contra; have: is_inv (TInv p_s).
-        by rewrite is_inv_TInv; case: (p_s) => // in Hnoncep_s *.
-      by rewrite -contra; case: (p_u) => // in Hnoncep_u *.
-    by iApply (public_opaque_secret _ (nonce_Nmul Hnoncep_u) (nonce_Nmul Hnoncep_s) p_u_s p_u_sV) => //.
+        by rewrite (is_inv_TInv (TNonce p_s) (negb_is_mul_nonce p_s)).
+      by rewrite -contra; case: (p_u) => //.
+    by iApply (public_opaque_secret _ (negb_is_mul_nonce p_u) (negb_is_mul_nonce p_s) p_u_s p_u_sV) => //.
   - do !iSplit => //.
     iApply (public_THashIS with "HpredSK") => //.
     rewrite minted_of_list.
@@ -198,7 +198,7 @@ iSplit.
   rewrite !elem_of_cons /β'.
   split.
     by right; left.
-  apply: subterm_TExp_exp; [done | exact: (nonce_Nmul Hnoncer) | exact: STRefl].
+  apply: subterm_TExp_exp; [done | exact: (negb_is_mul_nonce r) | exact: STRefl].
 - rewrite minted_of_list /=
       minted_THash minted_tag minted_of_list /=
       !minted_THash !minted_tag !minted_of_list /=
